let..in construct in syntax, via PHOAS encoding

syntax.v
@@ -6,195 +6,244 @@ Set Implicit Arguments.
 Unset Strict Implicit.
 Unset Printing Implicit Defensive.
 
+(** sorts of expressions we know how to approximate 
+    - real numbers
+    - functions on closed real intervals
+    - (conjunctions/disjunctions of combinations of) comparison of reals
+ *)
+Inductive sort := REAL | FUN | BOOL.
 
-(** syntax for the expressions we know how to approximate *)
-Inductive expr :=
-| e_add: expr -> expr -> expr
-| e_sub: expr -> expr -> expr
-| e_mul: expr -> expr -> expr
-| e_fromZ: Z -> expr
-| e_fromQ: Q -> expr
-| e_zer: expr
-| e_one: expr
-| e_pi: expr
-| e_div: expr -> expr -> expr
-| e_sqrt: expr -> expr
-| e_cos: expr -> expr
-| e_abs: expr -> expr
-| e_eval: fxpr -> expr -> expr
-| e_integrate: fxpr -> expr -> expr -> expr
-with fxpr :=
-| f_add: fxpr -> fxpr -> fxpr
-| f_sub: fxpr -> fxpr -> fxpr
-| f_mul: fxpr -> fxpr -> fxpr
-| f_div: fxpr -> fxpr -> fxpr
-| f_sqrt: fxpr -> fxpr
-| f_id: fxpr
-| f_cst: expr -> fxpr
-| f_trunc: fxpr -> fxpr.         (* the identity, simply truncates the model *)
-Inductive bxpr :=
-| b_le: expr -> expr -> bxpr
-| b_lt: expr -> expr -> bxpr
-| b_conj: bxpr -> bxpr -> bxpr.
+(** syntax for the expressions we know how to approximate 
+    we use parameterised higher order abstract syntax (PHOAS) in order to have a let..in construct and be able to share subexpressions
+    [@term X S] intuitively contains terms of sort [S] with variables in [X]
+*)
+Inductive term {X: sort -> Type}: sort -> Type :=
+(* real expressions *)
+| e_add: term REAL -> term REAL -> term REAL
+| e_sub: term REAL -> term REAL -> term REAL
+| e_mul: term REAL -> term REAL -> term REAL
+| e_fromZ: Z -> term REAL
+| e_fromQ: Q -> term REAL
+| e_zer: term REAL
+| e_one: term REAL
+| e_pi: term REAL
+| e_div: term REAL -> term REAL -> term REAL
+| e_sqrt: term REAL -> term REAL
+| e_cos: term REAL -> term REAL
+| e_abs: term REAL -> term REAL
+| e_eval: term FUN -> term REAL -> term REAL
+| e_integrate: term FUN -> term REAL -> term REAL -> term REAL
+(* functional expressions *)
+| f_add: term FUN -> term FUN -> term FUN
+| f_sub: term FUN -> term FUN -> term FUN
+| f_mul: term FUN -> term FUN -> term FUN
+| f_div: term FUN -> term FUN -> term FUN
+| f_sqrt: term FUN -> term FUN
+| f_id: term FUN
+| f_cst: term REAL -> term FUN
+| f_trunc: term FUN -> term FUN         (* the identity, simply truncates the model *)
+(* boolean expressions *)
+| b_le: term REAL -> term REAL -> term BOOL
+| b_ge: term REAL -> term REAL -> term BOOL
+| b_lt: term REAL -> term REAL -> term BOOL
+    (* need b_ge and not b_gt because Rgt unfolds to Rlt while Rge does not unfold to Rle *)
+| b_disj: term BOOL -> term BOOL -> term BOOL
+| b_conj: term BOOL -> term BOOL -> term BOOL
+(* let..in and variable *)
+| t_var: forall {S}, X S -> term S
+| t_let: forall {S T}, term S -> (X S -> term T) -> term T.
 
-(** see expressions as constant functions *)
-Coercion f_cst: expr >-> fxpr.
-
-(** declaring structures to get nice notations on expressions *)
-Canonical Structure eOps0: Ops0 := {|
-  car := expr;
-  add := e_add;
-  sub := e_sub;
-  mul := e_mul;
-  zer := e_zer;
-  one := e_one;
-|}.
-Canonical Structure eOps1 := {|
-  ops0  := eOps0;
-  fromZ := e_fromZ;
-  div   := e_div;
-  sqrt  := e_sqrt;
-  cos   := e_cos;
-  abs   := e_abs;
-  pi    := e_pi;
-|}.
-
-Definition f_zer := f_cst 0.
-Definition f_one := f_cst 1.
-Canonical Structure fOps0: Ops0 := {|
-  car := fxpr;
-  add := f_add;
-  sub := f_sub;
-  mul := f_mul;
-  zer := f_zer;
-  one := f_one;
-|}.
-Definition f_pi := f_cst pi.
-Definition f_fromZ z := f_cst (fromZ z).
-(** fake value, not to be used... *)
-Definition f_dontuse (f: fxpr): fxpr. exact f. Qed.
-Canonical Structure fOps1: Ops1 := {|
-  ops0  := fOps0;
-  fromZ := f_fromZ;
-  div   := f_div;
-  sqrt  := f_sqrt;
-  pi    := f_pi;
-  (** cos, and abs, are not available on functions, only on scalars *)
-  cos   := f_dontuse;
-  abs   := f_dontuse;
-|}.
+(** closed terms: they act polymorphically in X *)
+Definition Term S := forall X, @term X S.
+(** (terms of sort T with a single variable of sort S would be represented by type 
+    [forall X, X S -> @term X T]) *)
 
 
 (** real number semantics of expressions  *)
-Fixpoint esem (e: expr): R :=
-  match e with
-  | e_add e f => esem e + esem f
-  | e_sub e f => esem e - esem f
-  | e_mul e f => esem e * esem f
-  | e_div e f => esem e / esem f
-  | e_sqrt e => sqrt (esem e)
-  | e_cos e => cos (esem e)
-  | e_abs e => abs (esem e)
+Definition rval S: Type := match S with REAL => R | FUN => (R -> R) | BOOL => Prop end.
+Fixpoint sem S (t: @term rval S): rval S :=
+  match t in term S return rval S with
+  | e_add e f => sem e + sem f
+  | e_sub e f => sem e - sem f
+  | e_mul e f => sem e * sem f
+  | e_div e f => sem e / sem f
+  | e_sqrt e => sqrt (sem e)
+  | e_cos e => cos (sem e)
+  | e_abs e => abs (sem e)
   | e_fromQ q => Q2R q
   | e_fromZ z => fromZ z
   | e_zer => 0
   | e_one => 1
   | e_pi => pi
-  | e_eval f x => fsem f (esem x)
-  | e_integrate f a b => RInt (fsem f) (esem a) (esem b)
-  end
-with fsem (e: fxpr) (x: R): R :=
-  match e with
-  | f_add e f => fsem e x + fsem f x
-  | f_sub e f => fsem e x - fsem f x
-  | f_mul e f => fsem e x * fsem f x
-  | f_div e f => fsem e x / fsem f x
-  | f_sqrt e => sqrt (fsem e x)
-  | f_id => x
-  | f_cst e => esem e
-  | f_trunc f => fsem f x
+  | e_eval f x => sem f (sem x)
+  | e_integrate f a b => RInt (sem f) (sem a) (sem b)
+  | f_add e f => (fun x => sem e x + sem f x)
+  | f_sub e f => (fun x => sem e x - sem f x)
+  | f_mul e f => (fun x => sem e x * sem f x)
+  | f_div e f => (fun x => sem e x / sem f x)
+  | f_sqrt e => (fun x => sqrt (sem e x))
+  | f_id => id
+  | f_cst e => (fun _ => sem e)
+  | f_trunc f => sem f
+  | b_le e f => sem e <= sem f
+  | b_ge e f => sem e >= sem f
+  | b_lt e f => sem e < sem f
+  | b_disj b c => sem b \/ sem c
+  | b_conj b c => sem b /\ sem c
+  | t_var _ x => x
+  | t_let _ _ x k => sem (k (sem x))
   end.
-Fixpoint bsem (b: bxpr): Prop :=
-  match b with
-  | b_le e f => esem e <= esem f
-  | b_lt e f => esem e < esem f
-  | b_conj b c => bsem b /\ bsem c
-  end.
+Definition sem' S (u: Term S): rval S := sem (u rval).
 
-Lemma VAR: R. exact R0. Qed.
 
+
+(** reification for the above syntax *)
+
+(* TODO: 
+   - avoid redundant reductions? 
+   - maximal sharing using let-ins? [need OCaml?]
+   - reify user's let-ins?          [need OCaml?]
+*)
 Arguments f_bin [_ _] _ _ _ _ /.
 Arguments f_unr [_ _] _ _ _ /.
-
-(* TODO: avoid redundant reductions? *)
+Lemma VAR: R. exact R0. Qed.
 Ltac ereify e :=
-  lazymatch
-    eval cbn beta iota delta
-         [ROps0 ROps1 f_Ops0 car ops0 zer one add sub mul div sqrt cos abs pi f_bin f_unr fromZ] in e
+  lazymatch e
   with
-  | R0 => constr:(e_zer)
-  | R1 => constr:(e_one)
-  | Rplus ?e ?f => let e:=ereify e in let f:=ereify f in constr:(e_add e f)
-  | Rminus ?e ?f => let e:=ereify e in let f:=ereify f in constr:(e_sub e f)
-  | Rmult ?e ?f => let e:=ereify e in let f:=ereify f in constr:(e_mul e f)
-  | Rdiv ?e ?f => let e:=ereify e in let f:=ereify f in constr:(e_div e f)
-  | R_sqrt.sqrt ?e => let e:=ereify e in constr:(e_sqrt e)
-  | Rtrigo_def.cos ?e => let e:=ereify e in constr:(e_cos e)
-  | Rabs ?e => let e:=ereify e in constr:(e_abs e)
-  | Q2R ?q => constr:(e_fromQ q)
-  | IZR ?z => constr:(e_fromZ z)
-  | Rtrigo1.PI => constr:(e_pi)
+  | R0 => uconstr:(e_zer)
+  | R1 => uconstr:(e_one)
+  | Rplus ?e ?f => let e:=ereify e in let f:=ereify f in uconstr:(e_add e f)
+  | Rminus ?e ?f => let e:=ereify e in let f:=ereify f in uconstr:(e_sub e f)
+  | Rmult ?e ?f => let e:=ereify e in let f:=ereify f in uconstr:(e_mul e f)
+  | Rdiv ?e ?f => let e:=ereify e in let f:=ereify f in uconstr:(e_div e f)
+  | R_sqrt.sqrt ?e => let e:=ereify e in uconstr:(e_sqrt e)
+  | Rtrigo_def.cos ?e => let e:=ereify e in uconstr:(e_cos e)
+  | Rabs ?e => let e:=ereify e in uconstr:(e_abs e)
+  | Q2R ?q => uconstr:(e_fromQ q)
+  | IZR ?z => uconstr:(e_fromZ z)
+  | Rtrigo1.PI => uconstr:(e_pi)
   | RInt ?f ?a ?b =>
     let a:=ereify a in
     let b:=ereify b in
     let x:=fresh "x" in
-    let fVAR:=constr:(f VAR) in
+    let fVAR:=eval cbn beta iota delta
+         [ROps0 ROps1 f_Ops0 car ops0 zer one add sub mul div sqrt cos abs pi f_bin f_unr fromZ] in (f VAR) in
     let f:=freify fVAR in
-    constr:(e_integrate f a b)
+    uconstr:(e_integrate f a b)
   | VAR => fail "variable occurs under an unsupported context"
   | ?e => fail "unrecognised expression:" e
   end
  with freify f :=
-    lazymatch
-      eval cbn beta iota delta
-       [ROps0 ROps1 f_Ops0 car ops0 zer one add sub mul div sqrt cos abs pi f_bin f_unr fromZ]
-      in f
-    with
-  | Rplus ?e ?f => let e:=freify e in let f:=freify f in constr:(f_add e f)
-  | Rminus ?e ?f => let e:=freify e in let f:=freify f in constr:(f_sub e f)
-  | Rmult ?e ?f => let e:=freify e in let f:=freify f in constr:(f_mul e f)
-  | Rdiv ?e ?f => let e:=freify e in let f:=freify f in constr:(f_div e f)
-  | R_sqrt.sqrt ?e => let e:=freify e in constr:(f_sqrt e)
-  | VAR => constr:(f_id)
-  | ?e => let e:=ereify e in constr:(f_cst e)
+    lazymatch f with
+  | Rplus ?e ?f => let e:=freify e in let f:=freify f in uconstr:(f_add e f)
+  | Rminus ?e ?f => let e:=freify e in let f:=freify f in uconstr:(f_sub e f)
+  | Rmult ?e ?f => let e:=freify e in let f:=freify f in uconstr:(f_mul e f)
+  | Rdiv ?e ?f => let e:=freify e in let f:=freify f in uconstr:(f_div e f)
+  | R_sqrt.sqrt ?e => let e:=freify e in uconstr:(f_sqrt e)
+  | VAR => uconstr:(f_id)
+  | ?e => let e:=ereify e in uconstr:(f_cst e)
     end.
 Ltac breify b :=
   lazymatch b with
-  | Rle ?e ?f => let e:=ereify e in let f:=ereify f in constr:(b_le e f)
-  | Rlt ?e ?f => let e:=ereify e in let f:=ereify f in constr:(b_lt e f)
-  | Rge ?f ?e => fail "Rge (>=) not supported, please rewrite into Rle first"
-    (* let e:=ereify e in let f:=ereify f in constr:(b_le e f) *)
-  | Rgt ?f ?e => let e:=ereify e in let f:=ereify f in constr:(b_lt e f)
-  | ?b /\ ?c => let b:=breify b in let c:=breify c in constr:(b_conj b c)
+  | ?e <= ?f <= ?g =>
+    let e:=ereify e in let f:=ereify f in let g:=ereify g in
+    uconstr:(t_let f (fun f => b_conj (b_le e (t_var f)) (b_le (t_var f) g)))
+  | ?e <= ?f < ?g =>
+    let e:=ereify e in let f:=ereify f in let g:=ereify g in
+    uconstr:(t_let f (fun f => b_conj (b_le e (t_var f)) (b_lt (t_var f) g)))
+  | ?e < ?f <= ?g =>
+    let e:=ereify e in let f:=ereify f in let g:=ereify g in
+    uconstr:(t_let f (fun f => b_conj (b_lt e (t_var f)) (b_le (t_var f) g)))
+  | ?e < ?f <= ?g =>
+    let e:=ereify e in let f:=ereify f in let g:=ereify g in
+    uconstr:(t_let f (fun f => b_conj (b_lt e (t_var f)) (b_lt (t_var f) g)))
+  | Rle ?e ?f => let e:=ereify e in let f:=ereify f in uconstr:(b_le e f)
+  | Rge ?e ?f => let e:=ereify e in let f:=ereify f in uconstr:(b_ge e f)
+  | Rlt ?e ?f => let e:=ereify e in let f:=ereify f in uconstr:(b_lt e f)
+  | Rgt ?f ?e => let e:=ereify e in let f:=ereify f in uconstr:(b_lt e f)
+  | ?b /\ ?c => let b:=breify b in let c:=breify c in uconstr:(b_conj b c)
+  | ?b \/ ?c => let b:=breify b in let c:=breify c in uconstr:(b_disj b c)
   end.
+Ltac reify_real e :=
+  let e := eval cbn beta iota delta
+                [ROps0 ROps1 f_Ops0 car ops0 zer one add sub mul div sqrt cos abs pi f_bin f_unr fromZ]
+           in e in
+  let e := ereify e in
+  constr:((fun X => e): Term REAL).
+Ltac reify_fun e :=
+  let e := eval cbn beta iota delta
+                [ROps0 ROps1 f_Ops0 car ops0 zer one add sub mul div sqrt cos abs pi f_bin f_unr fromZ]
+           in e in
+  let e := freify e in
+  constr:((fun X => e): Term FUN).
+Ltac reify_prop e :=
+  let e := eval cbn beta iota delta
+                [ROps0 ROps1 f_Ops0 car ops0 zer one add sub mul div sqrt cos abs pi f_bin f_unr fromZ]
+           in e in
+  let e := breify e in
+  constr:((fun X => e): Term BOOL).
 
+(* tests for the above reification tatics *)
 (*
 Goal True.
-  let e := ereify constr:(Rplus R0 R1) in idtac e.
-  let e := ereify constr:(42) in idtac e.
-  let e := ereify constr:(4.2) in idtac e.
-  let e := ereify constr:(0+1: R) in idtac e.
-  let e := ereify constr:(RInt (fun z => z) R0 R1) in idtac e.
-  let e := ereify constr:(RInt (fun z => R0) R0 R1) in idtac e.
-  let e := ereify constr:(RInt (fun z => R0+z) R0 R1) in idtac e.
-  let e := ereify constr:(RInt (fun z => R0+z) R0 R1) in idtac e.
-  let e := ereify constr:(RInt (@sqrt _) R0 R1) in idtac e.
-  let e := ereify constr:(RInt (@sqrt _ + @sqrt _) R0 R1) in idtac e.
-  let e := ereify constr:(RInt (fun z => R0+z+cos (1/fromZ 2)) R0 R1) in idtac e.
-  let b := breify constr:(4 < 5 /\ RInt id 3.3 4.4 <= 18.9) in idtac b. 
-  let b := breify constr:(4 < 5 <= 6) in idtac b. (* TODO: improve with a let to share the middle term *)
-  let b := breify constr:(4 >= 5) in idtac b. 
+  let e := reify_real constr:(Rplus R0 R1) in pose e.
+  let e := reify_real constr:(42) in pose e.
+  let e := reify_real constr:(4.2) in pose e.
+  let e := reify_real constr:(0+1: R) in pose e.
+  let e := reify_real constr:(RInt (fun z => z) R0 R1) in pose e.
+  let e := reify_real constr:(RInt (fun z => R0) R0 R1) in pose e.
+  let e := reify_real constr:(RInt (fun z => R0+z) R0 R1) in pose e.
+  let e := reify_real constr:(RInt (fun z => R0+z) R0 R1) in pose e.
+  let e := reify_real constr:(RInt (@sqrt _) R0 R1) in pose e.
+  let e := reify_real constr:(RInt (@sqrt _ + @sqrt _) R0 R1) in pose e.
+  let e := reify_real constr:(RInt (fun z => R0+z+cos (1/fromZ 2)) R0 R1) in pose e.
+  let b := reify_prop constr:(4 <= 5 <= 6) in pose b.
+  let b := reify_prop constr:(4 < 5 /\ RInt id 3.3 4.4 <= 18.9) in pose b.
+  let b := reify_prop constr:(4 >= 5) in idtac b. 
 *)
+
+(** parametricity relation for terms.
+    This inductive relation is required because of our PHOAS encoding of the syntax.
+    We use it to be able to proceed by induction on terms when proving correctness of the interval/model semantics below. *)
+Inductive trel X Y (R: forall S, X S -> Y S -> Prop): forall S, @term X S -> @term Y S -> Prop :=
+| re_add: forall x y, trel R x y -> forall x' y', trel R x' y' -> trel R (e_add x x') (e_add y y')
+| re_sub: forall x y, trel R x y -> forall x' y', trel R x' y' -> trel R (e_sub x x') (e_sub y y')
+| re_mul: forall x y, trel R x y -> forall x' y', trel R x' y' -> trel R (e_mul x x') (e_mul y y')
+| re_fromZ: forall z, trel R (e_fromZ z) (e_fromZ z)
+| re_fromQ: forall q, trel R (e_fromQ q) (e_fromQ q)
+| re_zer: trel R e_zer e_zer
+| re_one: trel R e_one e_one
+| re_pi: trel R e_pi e_pi
+| re_div: forall x y, trel R x y -> forall x' y', trel R x' y' -> trel R (e_div x x') (e_div y y')
+| re_sqrt: forall x y, trel R x y -> trel R (e_sqrt x) (e_sqrt y)
+| re_cos: forall x y, trel R x y -> trel R (e_cos x) (e_cos y)
+| re_abs: forall x y, trel R x y -> trel R (e_abs x) (e_abs y)
+| re_eval: forall x y, trel R x y -> forall x' y', trel R x' y' -> trel R (e_eval x x') (e_eval y y')
+| re_integrate: forall f g, trel R f g -> forall x y, trel R x y -> forall x' y', trel R x' y' -> trel R (e_integrate f x x') (e_integrate g y y')
+| rf_add: forall x y, trel R x y -> forall x' y', trel R x' y' -> trel R (f_add x x') (f_add y y')
+| rf_sub: forall x y, trel R x y -> forall x' y', trel R x' y' -> trel R (f_sub x x') (f_sub y y')
+| rf_mul: forall x y, trel R x y -> forall x' y', trel R x' y' -> trel R (f_mul x x') (f_mul y y')
+| rf_div: forall x y, trel R x y -> forall x' y', trel R x' y' -> trel R (f_div x x') (f_div y y')
+| rf_sqrt: forall x y, trel R x y -> trel R (f_sqrt x) (f_sqrt y)
+| rf_id: trel R f_id f_id
+| rf_cst: forall x y, trel R x y -> trel R (f_cst x) (f_cst y)
+| rf_trunc: forall x y, trel R x y -> trel R (f_trunc x) (f_trunc y)
+| rb_le: forall x y, trel R x y -> forall x' y', trel R x' y' -> trel R (b_le x x') (b_le y y')
+| rb_ge: forall x y, trel R x y -> forall x' y', trel R x' y' -> trel R (b_ge x x') (b_ge y y')
+| rb_lt: forall x y, trel R x y -> forall x' y', trel R x' y' -> trel R (b_lt x x') (b_lt y y')
+| rb_disj: forall x y, trel R x y -> forall x' y', trel R x' y' -> trel R (b_disj x x') (b_disj y y')
+| rb_conj: forall x y, trel R x y -> forall x' y', trel R x' y' -> trel R (b_conj x x') (b_conj y y')
+| rt_var: forall S x y, R S x y -> trel R (t_var x) (t_var y)
+| rt_let: forall S T x y h k, trel R x y -> (forall a b, R S a b -> trel R (h a) (k b)) -> trel R (t_let x h) (@t_let _ _ T y k).
+
+(** all (closed) terms are parametric in the following sense, 
+    but this cannot be proved once and for all. Given a concrete closed term, it is however trivial to prove its parametricity (tactic: repeat (constructor; auto)) 
+    once a closed term has been proved parametric, one can prove facts by induction on this term
+    (see lemmas [Static.correct] and [Dynamic.correct] below) *)
+Definition parametric S (u: Term S) :=
+  forall X Y (R: forall S, X S -> Y S -> Prop), trel R (u X) (u Y).
+
+
 
 (** ** static evaluation strategy, where we fix a basis once and for all  *)
 Module Static.
@@ -205,101 +254,124 @@ Context {N: NBH} (MO: ModelOps) lo hi (M: Model MO lo hi).
 (** interpolation degree for divisions, square roots, and truncations *)
 Variable deg: Z.
 
-(** approximation of an expression using intervals / models *)
-Fixpoint eSem (e: expr): E II :=
-  match e with
-  | e_add e f => e_map2 (@add _) (eSem e) (eSem f)
-  | e_sub e f => e_map2 (@sub _) (eSem e) (eSem f)
-  | e_mul e f => e_map2 (@mul _) (eSem e) (eSem f)
-  | e_div e f => e_map2 (@div _) (eSem e) (eSem f)
-  | e_sqrt e => e_map (@sqrt _) (eSem e)
-  | e_cos e => e_map (@cos _) (eSem e)
-  | e_abs e => e_map (@abs _) (eSem e)
+
+(** interpretation of expressions using intervals / models / booleans *)
+Definition sval S :=
+  match S with
+  | REAL => E II
+  | FUN => E MM
+  | BOOL => E bool
+  end.
+Fixpoint Sem S (t: @term sval S): sval S :=
+  match t in term S return sval S with
+  | e_add e f => e_map2 (@add _) (Sem e) (Sem f)
+  | e_sub e f => e_map2 (@sub _) (Sem e) (Sem f)
+  | e_mul e f => e_map2 (@mul _) (Sem e) (Sem f)
+  | e_div e f => e_map2 (@div _) (Sem e) (Sem f)
+  | e_sqrt e => e_map (@sqrt _) (Sem e)
+  | e_cos e => e_map (@cos _) (Sem e)
+  | e_abs e => e_map (@abs _) (Sem e)
   | e_fromQ q => ret (fromQ q)
   | e_fromZ z => ret (fromZ z)
   | e_pi => ret pi
   | e_zer => ret 0
   | e_one => ret 1
   | e_eval f x => 
-      LET f ::= fSem f IN
-      LET x ::= eSem x IN 
+      LET f ::= Sem f IN
+      LET x ::= Sem x IN 
       meval f x
   | e_integrate f a b => 
-      LET f ::= fSem f IN 
-      LET a ::= eSem a IN 
-      LET b ::= eSem b IN 
+      LET f ::= Sem f IN 
+      LET a ::= Sem a IN 
+      LET b ::= Sem b IN 
       mintegrate f (Some a) (Some b)
-  end
-with fSem (e: fxpr): E MM :=
-  match e with
-  | f_add e f => e_map2 (@add _) (fSem e) (fSem f)
-  | f_sub e f => e_map2 (@sub _) (fSem e) (fSem f)
-  | f_mul e f => e_map2 (@mul _) (fSem e) (fSem f)
-  | f_div e f => LET e ::= fSem e IN LET f ::= fSem f IN mdiv deg e f
-  | f_sqrt e => LET e ::= fSem e IN msqrt deg e
+  | f_add e f => e_map2 (@add _) (Sem e) (Sem f)
+  | f_sub e f => e_map2 (@sub _) (Sem e) (Sem f)
+  | f_mul e f => e_map2 (@mul _) (Sem e) (Sem f)
+  | f_div e f => LET e ::= Sem e IN LET f ::= Sem f IN mdiv deg e f
+  | f_sqrt e => LET e ::= Sem e IN msqrt deg e
   | f_id => ret mid
-  | f_cst e => e_map mcst (eSem e)
-  | f_trunc e => e_map (mtruncate (Z.to_nat deg)) (fSem e)
+  | f_cst e => e_map mcst (Sem e)
+  | f_trunc e => e_map (mtruncate (Z.to_nat deg)) (Sem e)
+  | b_le e f => e_map2 is_le (Sem e) (Sem f)
+  | b_ge f e => e_map2 is_le (Sem e) (Sem f)
+  | b_lt e f => e_map2 is_lt (Sem e) (Sem f)
+  | b_disj b c => LET b ::= Sem b IN if b then ret true else Sem c
+  | b_conj b c => LET b ::= Sem b IN if b then Sem c else ret false
+  | t_var _ x => x
+  | t_let _ _ x k => Sem (k (Sem x))
   end.
-Fixpoint bSem (b: bxpr): E bool :=
-  match b with
-  | b_le e f => e_map2 is_le (eSem e) (eSem f)
-  | b_lt e f => e_map2 is_lt (eSem e) (eSem f)
-  | b_conj b c => e_map2 andb (bSem b) (bSem c)
+Definition Sem' S (u: Term S): sval S := Sem (u sval).
+
+(** correctness of the above semantics
+    the key lemma, [correct], is proved by induction on the parametricity relation *)
+Definition cval S: sval S -> rval S -> Prop :=
+  match S with
+  | REAL => EP' contains
+  | FUN  => EP' mcontains
+  | BOOL => EP' (fun b (P: Prop) => (is_true b -> P))
   end.
-
-Lemma econtains (e: expr): EP' contains (eSem e) (esem e)
-with fcontains (f: fxpr): EP' mcontains (fSem f) (fsem f).
+Lemma correct S (u: term S) (v: term S): trel cval u v -> cval (Sem u) (sem v).
 Proof.
-  - destruct e; simpl.
-    -- eapply ep_map2; try apply econtains; rel. 
-    -- eapply ep_map2; try apply econtains; rel. 
-    -- eapply ep_map2; try apply econtains; rel. 
-    -- constructor. rel. 
-    -- constructor. apply rfromQ. 
-    -- constructor. apply rzer.
-    -- constructor. apply rone.
-    -- constructor. rel.
-    -- eapply ep_map2; try apply econtains; rel. 
-    -- eapply ep_map; try apply econtains; rel. 
-    -- eapply ep_map; try apply econtains; rel. 
-    -- eapply ep_map; try apply econtains; rel. 
-    -- eapply ep_bind=>[F Ff|]. 2: apply fcontains. 
-       eapply ep_bind=>[X Xx|]. 2: apply econtains.  
-       by apply rmeval.
-    -- eapply ep_bind=>[F Ff|]. 2: apply fcontains.  
-       eapply ep_bind=>[A Aa|]. 2: apply econtains.  
-       eapply ep_bind=>[B Bb|]. 2: apply econtains.  
-       apply rmintegrate; rel. 
-  - destruct f; simpl.
-    -- eapply ep_map2; try apply fcontains. intros. by apply (radd (r:=mcontains)). 
-    -- eapply ep_map2; try apply fcontains. intros. by apply (rsub (r:=mcontains)). 
-    -- eapply ep_map2; try apply fcontains. intros. by apply (rmul (r:=mcontains)). 
-    -- eapply ep_bind=>[F Ff|]. 2: apply fcontains. 
-       eapply ep_bind=>[G Gg|]. 2: apply fcontains.  
-       by apply rmdiv.
-    -- eapply ep_bind=>[F Ff|]. 2: apply fcontains. 
-       by apply rmsqrt.
-    -- constructor. apply rmid.          
-    -- eapply ep_map; try apply econtains. intros. by apply rmcst.          
-    -- eapply ep_map; try apply fcontains. intros. by apply rmtruncate.          
-Qed.
-Fixpoint bcontains (b: bxpr): EP' (fun b (P: Prop) => (is_true b -> P)) (bSem b) (bsem b).
-Proof.
-  induction b; cbn.
-  -- eapply ep_map2; try apply econtains. intros ??. case is_leE=>//. auto.  
-  -- eapply ep_map2; try apply econtains. intros ??. case is_ltE=>//. auto.
-  -- eapply ep_map2; try apply bcontains. move=>??/=??/andP[??]. auto. 
+  induction 1; cbn.
+  - eapply ep_map2; eauto. rel. 
+  - eapply ep_map2; eauto. rel. 
+  - eapply ep_map2; eauto. rel. 
+  - constructor. rel. 
+  - constructor. apply rfromQ. 
+  - constructor. rel. 
+  - constructor. rel. 
+  - constructor. rel.
+  - eapply ep_map2; eauto. rel. 
+  - eapply ep_map; eauto. rel. 
+  - eapply ep_map; eauto. rel. 
+  - eapply ep_map; eauto. rel. 
+  - eapply ep_bind=>[F Ff|]; eauto. 
+    eapply ep_bind=>[X Xx|]; eauto.
+    by apply rmeval.
+  - eapply ep_bind=>[F Ff|]; eauto.  
+    eapply ep_bind=>[A Aa|]; eauto.  
+    eapply ep_bind=>[B Bb|]; eauto.  
+    apply rmintegrate; rel. 
+  - eapply ep_map2; eauto. intros. by apply (radd (r:=mcontains)). 
+  - eapply ep_map2; eauto. intros. by apply (rsub (r:=mcontains)). 
+  - eapply ep_map2; eauto. intros. by apply (rmul (r:=mcontains)). 
+  - eapply ep_bind=>[F Ff|]; eauto. 
+    eapply ep_bind=>[G Gg|]; eauto.
+    by apply rmdiv.
+  - eapply ep_bind=>[F Ff|]; eauto.
+    by apply rmsqrt.
+  - constructor. apply rmid.          
+  - eapply ep_map; eauto. intros. by apply rmcst.          
+  - eapply ep_map; eauto. intros. by apply rmtruncate.
+  - eapply ep_map2; eauto. intros ??. case is_leE=>//. auto.  
+  - eapply ep_map2; eauto. intros ??. case is_leE=>//. auto using Rle_ge. 
+  - eapply ep_map2; eauto. intros ??. case is_ltE=>//. auto.
+  - eapply ep_bind=>[b|]; eauto. 
+    case b. constructor. left; auto. intros _.
+    case: IHtrel2=>//. constructor. right; auto.
+  - eapply ep_bind=>[b|]; eauto. 
+    case b. case: IHtrel2=>//. constructor. auto. by constructor.
+  - assumption.
+  - auto. 
 Qed.
 
+(** correctness on parametric (closed) terms follows *)
+Lemma Correct: forall S (u: Term S), parametric u -> cval (Sem' u) (sem' u).
+Proof. intros S u U. apply correct, U. Qed.
+
+  
 (** small corollary, useful to obtain a tactic in tactic.v *)
-Lemma check b: (let b := bSem b in
-                match b with ret b => is_true b | err s => False end) ->
-               bsem b.
-Proof. by case bcontains. Qed.
+Lemma check (b: Term BOOL):
+  parametric b ->
+  (let b := Sem' b in
+   match b with ret b => is_true b | err s => False end) ->
+  sem' b.
+Proof. move: (@Correct BOOL)=>/= C B. by case C. Qed.
 
 End s.
 Arguments check {_ _ _ _} _ _ _ _.
+Arguments Sem {_} _ _ [_] _.
 
 End Static.
 
@@ -313,106 +385,223 @@ Context {N: NBH} (MO: II -> II -> ModelOps) (M: forall D: Domain, Model (MO dlo 
 (** interpolation degree for divisions and square roots *)
 Variable deg: Z.
 
-(** approximation of an expression using intervals / models *)
-Fixpoint eSem (e: expr): E II :=
-  match e with
-  | e_add e f => e_map2 (@add _) (eSem e) (eSem f)
-  | e_sub e f => e_map2 (@sub _) (eSem e) (eSem f)
-  | e_mul e f => e_map2 (@mul _) (eSem e) (eSem f)
-  | e_div e f => e_map2 (@div _) (eSem e) (eSem f)
-  | e_sqrt e => e_map (@sqrt _) (eSem e)
-  | e_cos e => e_map (@cos _) (eSem e)
-  | e_abs e => e_map (@abs _) (eSem e)
+(** interpretation of expressions using intervals / models / booleans *)
+Definition sval S :=
+  match S with
+  | REAL => E II
+  | FUN => (forall MO: ModelOps, E MM)
+  | BOOL => E bool
+  end.
+Fixpoint Sem S (t: @term sval S): sval S :=
+  match t in term S return sval S with
+  | e_add e f => e_map2 (@add _) (Sem e) (Sem f)
+  | e_sub e f => e_map2 (@sub _) (Sem e) (Sem f)
+  | e_mul e f => e_map2 (@mul _) (Sem e) (Sem f)
+  | e_div e f => e_map2 (@div _) (Sem e) (Sem f)
+  | e_sqrt e => e_map (@sqrt _) (Sem e)
+  | e_cos e => e_map (@cos _) (Sem e)
+  | e_abs e => e_map (@abs _) (Sem e)
   | e_fromQ q => ret (fromQ q)
   | e_fromZ z => ret (fromZ z)
   | e_pi => ret pi
   | e_zer => ret 0
   | e_one => ret 1
   | e_eval f x => err "evaluation not yet supported in dynamic mode"
-      (* LET f ::= fSem f IN *)
-      (* LET x ::= eSem x IN  *)
+      (* LET f ::= Sem f IN *)
+      (* LET x ::= Sem x IN  *)
       (* meval f x *)
   | e_integrate f a b => 
-      LET a ::= eSem a IN 
-      LET b ::= eSem b IN 
+      LET a ::= Sem a IN 
+      LET b ::= Sem b IN 
       if ~~ is_lt a b then err "dynamic: integral does not yield a valid domain" else
-      LET f ::= @fSem (MO a b) f IN 
+      LET f ::= Sem f (MO a b) IN 
       mintegrate f None None
-  end
-with fSem {MO: ModelOps} (e: fxpr): E MM :=
-  match e with
-  | f_add e f => e_map2 (@add _) (fSem e) (fSem f)
-  | f_sub e f => e_map2 (@sub _) (fSem e) (fSem f)
-  | f_mul e f => e_map2 (@mul _) (fSem e) (fSem f)
-  | f_div e f => LET e ::= fSem e IN LET f ::= fSem f IN mdiv deg e f  (** note the degree used here *)
-  | f_sqrt e => LET e ::= fSem e IN msqrt deg e (** note the degree used here *)
-  | f_id => ret mid
-  | f_cst e => e_map mcst (eSem e)
-  | f_trunc e => e_map (mtruncate (Z.to_nat deg)) (fSem e) (** note the degree used here *)
+  | f_add e f => fun MO => e_map2 (@add _) (Sem e MO) (Sem f MO)
+  | f_sub e f => fun MO => e_map2 (@sub _) (Sem e MO) (Sem f MO)
+  | f_mul e f => fun MO => e_map2 (@mul _) (Sem e MO) (Sem f MO)
+  | f_div e f => fun MO => LET e ::= Sem e MO IN LET f ::= Sem f MO IN mdiv deg e f
+  | f_sqrt e => fun MO => LET e ::= Sem e MO IN msqrt deg e
+  | f_id => fun MO => ret mid
+  | f_cst e => fun MO => e_map mcst (Sem e)
+  | f_trunc e => fun MO => e_map (mtruncate (Z.to_nat deg)) (Sem e MO)
+  | b_le e f => e_map2 is_le (Sem e) (Sem f)
+  | b_ge f e => e_map2 is_le (Sem e) (Sem f)
+  | b_lt e f => e_map2 is_lt (Sem e) (Sem f)
+  | b_disj b c => LET b ::= Sem b IN if b then ret true else Sem c
+  | b_conj b c => LET b ::= Sem b IN if b then Sem c else ret false
+  | t_var _ x => x
+  | t_let _ _ x k => Sem (k (Sem x))
   end.
-Fixpoint bSem (b: bxpr): E bool :=
-  match b with
-  | b_le e f => e_map2 is_le (eSem e) (eSem f)
-  | b_lt e f => e_map2 is_lt (eSem e) (eSem f)
-  | b_conj b c => e_map2 andb (bSem b) (bSem c)
-  end.
+Definition Sem' S (u: Term S): sval S := Sem (u sval).
 
-Lemma econtains (e: expr): EP' contains (eSem e) (esem e)
-with fcontains {MO' a b} {M': Model MO' a b}(f: fxpr): EP' mcontains (fSem f) (fsem f).
+(** correctness of the above semantics
+    the key lemma, [correct], is proved by induction on the parametricity relation *)
+Definition cval S: sval S -> rval S -> Prop :=
+  match S with
+  | REAL => EP' contains
+  | FUN  => fun F f => forall MO a b (M: Model MO a b), EP' M (F MO) f
+  | BOOL => EP' (fun b (P: Prop) => (is_true b -> P))
+  end.
+Lemma correct S (u: term S) (v: term S): trel cval u v -> cval (Sem u) (sem v).
 Proof.
-  - destruct e; simpl.
-    -- eapply ep_map2; try apply econtains; rel. 
-    -- eapply ep_map2; try apply econtains; rel. 
-    -- eapply ep_map2; try apply econtains; rel. 
-    -- constructor. rel. 
-    -- constructor. apply rfromQ. 
-    -- constructor. apply rzer.
-    -- constructor. apply rone.
-    -- constructor. rel. 
-    -- eapply ep_map2; try apply econtains; rel. 
-    -- eapply ep_map; try apply econtains; rel. 
-    -- eapply ep_map; try apply econtains; rel. 
-    -- eapply ep_map; try apply econtains; rel. 
-    -- constructor. 
-       (* eapply ep_bind=>[F Ff|]. 2: apply fcontains.  *)
-       (* eapply ep_bind=>[X Xx|]. 2: apply econtains.   *)
-       (* by apply rmeval. *)
-    -- eapply ep_bind=>[A Aa|]. 2: apply econtains.  
-       eapply ep_bind=>[B Bb|]. 2: apply econtains.
-       case_eq (is_lt A B)=>[ab|]. 2: constructor.
-       specialize (fcontains _ _ _ (M (DfromI2 Aa Bb ab))).
-       eapply ep_bind=>[F Ff|]. 2: apply fcontains.
-       eapply rmintegrate; first apply Ff; by constructor. 
-  - destruct f; simpl.
-    -- eapply ep_map2; try apply fcontains. intros. by apply (radd (r:=mcontains)). 
-    -- eapply ep_map2; try apply fcontains. intros. by apply (rsub (r:=mcontains)). 
-    -- eapply ep_map2; try apply fcontains. intros. by apply (rmul (r:=mcontains)). 
-    -- eapply ep_bind=>[F Ff|]. 2: apply fcontains. 
-       eapply ep_bind=>[G Gg|]. 2: apply fcontains.  
-       by apply rmdiv.
-    -- eapply ep_bind=>[F Ff|]. 2: apply fcontains. 
-       by apply rmsqrt.
-    -- constructor. apply rmid.          
-    -- eapply ep_map; try apply econtains. intros. by apply rmcst.          
-    -- eapply ep_map; try apply fcontains. intros. by apply rmtruncate.          
+  induction 1; cbn -[RInt];
+    try (intros MO' a b M';
+         try specialize (IHtrel  _ _ _ M');
+         try (specialize (IHtrel1  _ _ _ M'); specialize (IHtrel2  _ _ _ M'))).
+  - eapply ep_map2; eauto. rel. 
+  - eapply ep_map2; eauto. rel. 
+  - eapply ep_map2; eauto. rel. 
+  - constructor. rel. 
+  - constructor. apply rfromQ. 
+  - constructor. rel. 
+  - constructor. rel. 
+  - constructor. rel.
+  - eapply ep_map2; eauto. rel. 
+  - eapply ep_map; eauto. rel. 
+  - eapply ep_map; eauto. rel. 
+  - eapply ep_map; eauto. rel. 
+  - constructor. 
+    (* eapply ep_bind=>[F Ff|]; eauto.  *)
+    (* eapply ep_bind=>[X Xx|]; eauto. *)
+    (* by apply rmeval. *)
+  - eapply ep_bind=>[A Aa|]; eauto.  
+    eapply ep_bind=>[B Bb|]; eauto.  
+    case_eq (is_lt A B)=>[ab|]. 2: constructor.
+    specialize (IHtrel1 _ _ _ (M (DfromI2 Aa Bb ab))).
+    eapply ep_bind=>[F Ff|]; eauto.
+    eapply rmintegrate; first apply Ff; by constructor. 
+  - eapply ep_map2; eauto. intros. by apply (radd (r:=mcontains)).
+  - eapply ep_map2; eauto. intros. by apply (rsub (r:=mcontains)).
+  - eapply ep_map2; eauto. intros. by apply (rmul (r:=mcontains)). 
+  - eapply ep_bind=>[F Ff|]; eauto. 
+    eapply ep_bind=>[G Gg|]; eauto.
+    by apply rmdiv.
+  - eapply ep_bind=>[F Ff|]; eauto.
+    by apply rmsqrt.
+  - constructor. apply rmid.          
+  - eapply ep_map; eauto. intros. by apply rmcst.          
+  - eapply ep_map; eauto. intros. by apply rmtruncate.          
+  - eapply ep_map2; eauto. intros ??. case is_leE=>//. auto.  
+  - eapply ep_map2; eauto. intros ??. case is_leE=>//. auto using Rle_ge. 
+  - eapply ep_map2; eauto. intros ??. case is_ltE=>//. auto.
+  - eapply ep_bind=>[b|]; eauto. 
+    case b. constructor. left; auto. intros _.
+    case: IHtrel2=>//. constructor. right; auto.
+  - eapply ep_bind=>[b|]; eauto. 
+    case b. case: IHtrel2=>//. constructor. auto. by constructor.
+  - assumption.
+  - auto. 
 Qed.
 
-Fixpoint bcontains (b: bxpr): EP' (fun b (P: Prop) => (is_true b -> P)) (bSem b) (bsem b).
-Proof.
-  induction b; cbn.
-  -- eapply ep_map2; try apply econtains. intros ??. case is_leE=>//. auto.  
-  -- eapply ep_map2; try apply econtains. intros ??. case is_ltE=>//. auto.
-  -- eapply ep_map2; try apply bcontains. move=>??/=??/andP[??]. auto. 
-Qed.
+(** correctness on parametric (closed) terms follows *)
+Lemma Correct: forall S (u: Term S), parametric u -> cval (Sem' u) (sem' u).
+Proof. intros S u U. apply correct, U. Qed.
 
+  
 (** small corollary, useful to obtain a tactic in tactic.v *)
-Lemma check b: (let b := bSem b in
-                match b with ret b => is_true b | err s => False end) ->
-               bsem b.
-Proof. by case bcontains. Qed.
+Lemma check (b: Term BOOL):
+  parametric b ->
+  (let b := Sem' b in
+   match b with ret b => is_true b | err s => False end) ->
+  sem' b.
+Proof. move: (@Correct BOOL)=>/= C B. by case C. Qed.
 
 End s.
 Arguments check {_ _} _ _ _.
-Arguments fSem {_} _ _ _ _.
 
 End Dynamic.
+
+
+(** below: notations for expressions
+    mostly used for tests in tests.v for now 
+    sadly, trying to declare canonical structures of Ops0, Ops1, raises universe inconsistencies
+ *)
+
+Definition expr X := @term X REAL.
+Definition fxpr X := @term X FUN.
+Definition bxpr X := @term X BOOL.
+
+Declare Scope expr_scope.
+Bind Scope expr_scope with expr.
+Delimit Scope expr_scope with expr.
+Definition e_add' X: expr X -> expr X -> expr X := e_add.
+Definition e_sub' X: expr X -> expr X -> expr X := e_sub.
+Definition e_mul' X: expr X -> expr X -> expr X := e_mul.
+Definition e_div' X: expr X -> expr X -> expr X := e_div.
+Infix "+" := e_add': expr_scope. 
+Infix "-" := e_sub': expr_scope.
+Infix "*" := e_mul': expr_scope.
+Infix "/" := e_div': expr_scope.
+Notation "0" := e_zer: expr_scope.
+Notation "1" := e_one: expr_scope.
+Definition fromQ' {X}: Q -> expr X := e_fromQ.
+Definition fromZ' {X}: Z -> expr X := e_fromZ.
+Definition sqrt' {X}: expr X -> expr X := e_sqrt.
+Definition cos' {X}: expr X -> expr X := e_cos.
+Definition abs' {X}: expr X -> expr X:= e_abs.
+Definition pi' {X}: expr X := e_pi.
+
+Definition cst' X: expr X -> fxpr X := f_cst.
+Coercion cst': expr >-> fxpr.
+Declare Scope fxpr_scope.
+Bind Scope fxpr_scope with fxpr.
+Delimit Scope fxpr_scope with fxpr.
+Definition f_add' X: fxpr X -> fxpr X -> fxpr X := f_add.
+Definition f_sub' X: fxpr X -> fxpr X -> fxpr X := f_sub.
+Definition f_mul' X: fxpr X -> fxpr X -> fxpr X := f_mul.
+Definition f_div' X: fxpr X -> fxpr X -> fxpr X := f_div.
+Definition f_zer {X}: fxpr X := cst' 0. 
+Definition f_one {X}: fxpr X := cst' 1. 
+Infix "+" := f_add': fxpr_scope. 
+Infix "-" := f_sub': fxpr_scope.
+Infix "*" := f_mul': fxpr_scope.
+Infix "/" := f_div': fxpr_scope.
+Notation "0" := f_zer: fxpr_scope.
+Notation "1" := f_one: fxpr_scope.
+
+Definition integrate' X: fxpr X -> expr X -> expr X -> expr X := e_integrate.
+Definition eval' X: fxpr X -> expr X -> expr X := e_eval.
+Definition id' {X}: fxpr X := f_id.
+Definition truncate' X: fxpr X -> fxpr X := f_trunc.
+Definition fsqrt X: fxpr X -> fxpr X := f_sqrt.
+
+Declare Scope bxpr_scope.
+Bind Scope bxpr_scope with bxpr.
+Delimit Scope bxpr_scope with bxpr.
+Definition b_le' X: expr X -> expr X -> bxpr X := b_le.
+Definition b_ge' X: expr X -> expr X -> bxpr X := b_ge.
+Definition b_lt' X: expr X -> expr X -> bxpr X := b_lt.
+Definition b_gt' X e f: bxpr X := b_lt' f e.
+Definition b_conj' X: bxpr X -> bxpr X -> bxpr X := b_conj.
+Definition b_disj' X: bxpr X -> bxpr X -> bxpr X := b_disj.
+Infix "<=" := b_le': bxpr_scope. 
+Infix "<" := b_lt': bxpr_scope. 
+Infix ">=" := b_ge': bxpr_scope. 
+Infix ">" := b_gt': bxpr_scope. 
+Infix "/\" := b_conj': bxpr_scope. 
+Infix "\/" := b_disj': bxpr_scope.
+
+Definition let' {X S T}: @term X S -> (term S -> term T) -> term T :=
+  fun a k => t_let a (fun x => k (t_var x)). 
+Notation "'let_ee' x := e 'in' g" := (let' (e%expr: expr _) (fun (x: expr _) => (g%expr: expr _))) (at level 200, x binder, right associativity): expr_scope.
+Notation "'let_ef' x := e 'in' g" := (let' (e%expr: expr _) (fun (x: expr _) => (g%fxpr: fxpr _))) (at level 200, x binder, right associativity): fxpr_scope.
+Notation "'let_eb' x := e 'in' g" := (let' (e%expr: expr _) (fun (x: expr _) => (g%bxpr: bxpr _))) (at level 200, x binder, right associativity): bxpr_scope.
+Notation "'let_fe' x := e 'in' g" := (let' (e%fxpr: fxpr _) (fun (x: fxpr _) => (g%expr: expr _))) (at level 200, x binder, right associativity): expr_scope.
+Notation "'let_ff' x := e 'in' g" := (let' (e%fxpr: fxpr _) (fun (x: fxpr _) => (g%bxpr: fxpr _))) (at level 200, x binder, right associativity): fxpr_scope.
+Notation "'let_fb' x := e 'in' g" := (let' (e%fxpr: fxpr _) (fun (x: fxpr _) => (g%bxpr: bxpr _))) (at level 200, x binder, right associativity): bxpr_scope.
+Notation EXPR t := ((fun X => (t%expr: expr X)): Term REAL).
+Notation FXPR t := ((fun X => (t%fxpr: fxpr X)): Term FUN).
+Notation BXPR t := ((fun X => (t%bxpr: bxpr X)): Term BOOL).
+
+(*
+Check EXPR (1+e_pi).
+Check EXPR (1+integrate' id' 0 1).
+Check FXPR (id'/id').
+Check EXPR (1+integrate' (id' / fsqrt id') 0 (fromQ' 3.3)).
+Check EXPR (1+integrate' (id' / (fsqrt id' + fromQ' 3.2)) 0 (fromQ' 3.3)).
+Check EXPR (let_ee x := 1+e_pi in x + x).
+Check EXPR (let_ee x := 1+e_pi in x + let_ee y := x*x in sqrt' (y+y)).
+Check FXPR (let_ef x := 1+e_pi in id' + x).
+Check FXPR (let_ff f := 1-id' in id' * id').
+Check BXPR (1 <= 0 \/ cos' pi' < 1 /\ cos' 0 >= 1).
+*) 
